investigations/bedrock2/RiscvMachineWithCavaDevice/Bedrock2ToCava.v
@@ -1,0 +1,111 @@
+Require Import Coq.ZArith.ZArith.
+Require Import Coq.Lists.List. Import ListNotations.
+Require Import coqutil.Word.Interface coqutil.Map.Interface.
+Require Import coqutil.Map.OfListWord.
+Require Import coqutil.Datatypes.PropSet.
+Require Import riscv.Platform.MetricRiscvMachine.
+Require Import riscv.Utility.FreeMonad.
+Require Import riscv.Utility.runsToNonDet.
+Require Import riscv.Spec.Decode.
+Require Import riscv.Utility.InstructionCoercions.
+Require Import riscv.Platform.MetricSane.
+Require Import compiler.SeparationLogic.
+Require Import compiler.Pipeline.
+Require Import Bedrock2Experiments.StateMachineSemantics.
+Require Import Bedrock2Experiments.RiscvMachineWithCavaDevice.InternalMMIOMachine.
+Require Import Bedrock2Experiments.RiscvMachineWithCavaDevice.DetIncrMachine.
+Require Import Bedrock2Experiments.StateMachineMMIOSpec.
+Require Import Bedrock2Experiments.StateMachineMMIO.
+Require Import Bedrock2Experiments.RiscvMachineWithCavaDevice.MMIOToCava.
+
+Section WithParams.
+  Context {word : Interface.word.word 32} {word_ok: word.ok word}
+          {word_riscv_ok: RiscvWordProperties.word.riscv_ok word}
+          {Registers: map.map Z word} {Registers_ok: map.ok Registers}
+          {mem : Interface.map.map word Byte.byte} {mem_ok: map.ok mem}
+          {state_machine_params: StateMachineSemantics.parameters.parameters 32 word mem}
+          {state_machine_params_ok: StateMachineSemantics.parameters.ok state_machine_params}
+          {D: device}
+          (sched: schedule).
+
+  Open Scope ilist_scope.
+
+  Global Instance MMIO_compiler_params: StateMachineMMIO.MMIO.parameters := {|
+    MMIO.word := word;
+    MMIO.word_ok := _;
+    MMIO.word_riscv_ok := _;
+    MMIO.mem := SortedListWord.map _ _;
+    MMIO.mem_ok := _;
+    MMIO.locals := _;
+    MMIO.locals_ok := _;
+    MMIO.funname_env := SortedListString.map;
+    MMIO.funname_env_ok := SortedListString.ok;
+  |}.
+
+  Global Instance pipeline_params: Pipeline.parameters := {|
+    Pipeline.W := _;
+    Pipeline.mem := _;
+    Pipeline.Registers := _;
+    Pipeline.string_keyed_map := _;
+    Pipeline.ext_spec := StateMachineSemantics.ext_spec;
+    Pipeline.compile_ext_call :=
+      @FlatToRiscvDef.FlatToRiscvDef.compile_ext_call StateMachineMMIO.compilation_params;
+    Pipeline.M := _;
+    Pipeline.MM := _;
+    Pipeline.RVM := MetricMinimalMMIO.IsRiscvMachine;
+    Pipeline.PRParams := _
+  |}.
+
+  Definition regs_initialized(regs: Registers): Prop :=
+    forall r : Z, 0 < r < 32 -> exists v : word, map.get regs r = Some v.
+
+  (* similar to compiler.LowerPipeline.machine_ok, but takes an `ExtraRiscvMachine D` instead of
+     a `MetricRiscvMachine` *)
+  Definition machine_ok(p_functions: word)(f_entry_rel_pos: Z)(stack_start stack_pastend: word)
+             (finstrs: list Instruction)
+             (p_call pc: word)(mH: mem)(Rdata Rexec: mem -> Prop)(mach: ExtraRiscvMachine D): Prop :=
+      let CallInst := Jal RegisterNames.ra
+                          (f_entry_rel_pos + word.signed (word.sub p_functions p_call)) : Instruction in
+      (program RV32I p_functions finstrs *
+       program RV32I p_call [CallInst] *
+       LowerPipeline.mem_available stack_start stack_pastend *
+       Rdata * Rexec * eq mH
+      )%sep mach.(getMem) /\
+      subset (footpr (program RV32I p_functions finstrs *
+                      program RV32I p_call [CallInst] *
+                      Rexec)%sep)
+             (of_list (getXAddrs mach)) /\
+      word.unsigned (mach.(getPc)) mod 4 = 0 /\
+      mach.(getPc) = pc /\
+      mach.(getNextPc) = word.add mach.(getPc) (word.of_Z 4) /\
+      regs_initialized mach.(getRegs) /\
+      map.get mach.(getRegs) RegisterNames.sp = Some stack_pastend (*/\
+      TODO we should have some conditions that imply these, but don't use the notion of
+      MMIO, because MMIO is only used at the intermediate spec that we want to cancel out
+      map.undef_on m StateMachineSemantics.parameters.isMMIOAddr /\
+      disjoint (of_list xAddrs) StateMachineSemantics.parameters.isMMIOAddr *) .
+
+  Lemma bedrock2_and_cava_system_correct: forall functions instrs pos_map required_stack_space
+        f_entry_name fbody mc p_functions f_entry_rel_pos stack_start stack_pastend
+      finstrs p_call mH Rdata Rexec (initialL: ExtraRiscvMachine D) steps_done postH,
+      ExprImp.valid_funs functions ->
+      compile functions = Some (instrs, pos_map, required_stack_space) ->
+      map.get functions f_entry_name = Some ([], [], fbody) ->
+      map.get pos_map f_entry_name = Some f_entry_rel_pos ->
+      required_stack_space <= word.unsigned (word.sub stack_pastend stack_start) / bytes_per_word ->
+      Semantics.exec.exec functions fbody initialL.(getLog) mH map.empty mc
+           (fun t' m' l' mc' => postH m') ->
+      machine_ok p_functions f_entry_rel_pos stack_start stack_pastend finstrs p_call
+                 p_call mH Rdata Rexec initialL ->
+      exists steps_remaining finalL mH',
+        run_rec sched steps_done steps_remaining initialL = (Some tt, finalL) /\
+        machine_ok p_functions f_entry_rel_pos stack_start stack_pastend finstrs p_call
+                   (word.add p_call (word.of_Z 4)) mH' Rdata Rexec finalL /\
+        postH mH'.
+  Proof.
+    intros.
+    pose proof @Pipeline.compiler_correct as P.
+    pose proof stateMachine_to_cava as Q.
+  Admitted.
+
+End WithParams.
