investigations/bedrock2/RiscvMachineWithCavaDevice/MMIOToCava.v
@@ -1,0 +1,105 @@
+Require Import Coq.ZArith.ZArith.
+Require Import Coq.Lists.List. Import ListNotations.
+Require Import coqutil.Word.Interface coqutil.Map.Interface.
+Require Import coqutil.Map.OfListWord.
+Require Import coqutil.Datatypes.PropSet.
+Require Import Bedrock2Experiments.StateMachineSemantics.
+Require Import riscv.Platform.MetricRiscvMachine.
+Require Import riscv.Utility.FreeMonad.
+Require Import riscv.Utility.runsToNonDet.
+Require Import riscv.Platform.MetricSane.
+Require Import Bedrock2Experiments.RiscvMachineWithCavaDevice.InternalMMIOMachine.
+Require Import Bedrock2Experiments.RiscvMachineWithCavaDevice.DetIncrMachine.
+Require Import Bedrock2Experiments.StateMachineMMIOSpec.
+
+Section WithParams.
+  Context {word : Interface.word.word 32} {word_ok: word.ok word}
+          {Registers: map.map Z word} {Registers_ok: map.ok Registers}
+          {mem : Interface.map.map word Byte.byte} {mem_ok: map.ok mem}
+          {state_machine_params: StateMachineSemantics.parameters.parameters 32 word mem}
+          {state_machine_params_ok: StateMachineSemantics.parameters.ok state_machine_params}
+          {D: device}
+          (device_state_related: StateMachineSemantics.parameters.state -> D -> Prop).
+
+  Inductive related: MetricRiscvMachine -> ExtraRiscvMachine D -> Prop :=
+    mkRelated: forall regs pc npc m xAddrs (t: list LogItem) mc s d,
+      execution t s ->
+      device_state_related s d ->
+      map.undef_on m StateMachineSemantics.parameters.isMMIOAddr ->
+      disjoint (of_list xAddrs) StateMachineSemantics.parameters.isMMIOAddr ->
+      related
+        {| MetricRiscvMachine.getMachine :=
+             {| getRegs := regs;
+                getPc := pc;
+                getNextPc := npc;
+                getMem := m;
+                getXAddrs := xAddrs;
+                getLog := t; |};
+           getMetrics := mc; |}
+        {| ExtraRiscvMachine.getMachine :=
+             {| getRegs := regs;
+                getPc := pc;
+                getNextPc := npc;
+                getMem := m;
+                getXAddrs := xAddrs;
+                getLog := []; |};
+           getExtraState := d |}.
+
+  Definition stepH(initialL: MetricRiscvMachine)(post: MetricRiscvMachine -> Prop): Prop :=
+    free.interp MetricMinimalMMIO.interp_action (riscv.Platform.Run.run1 Decode.RV32I)
+                initialL (fun _ : unit => post).
+
+  Variable sched: schedule.
+
+  Lemma stateMachine_to_cava_1: forall (initialH: MetricRiscvMachine) (initialL: ExtraRiscvMachine D)
+                                       steps_done post,
+      related initialH initialL ->
+      stepH initialH post ->
+      exists finalL finalH, nth_step sched steps_done initialL = (Some tt, finalL) /\
+                            related finalH finalL /\
+                            post finalH.
+  Proof.
+    intros.
+    unfold stepH in H0.
+    unfold nth_step.
+    (*
+      above the line:
+      Run.run1 with Bedrock2Experiments.Riscv.MetricMinimalMMIO.IsRiscvMachine
+      below the line:
+      Run.run1 with Bedrock2Experiments.RiscvMachineWithCavaDevice.InternalMMIOMachine.IsRiscvMachine
+
+      would like to say "forall monadic programs, L behaves like H" --> L needs to go through
+      monad materialization as well *)
+
+    (* not sure if useful: *)
+    pose proof (run1_sane Decode.RV32I) as A.
+    unfold MetricPrimitives.mcomp_sane, Primitives.mcomp_sat, Primitives.valid_machine,
+        MetricMinimalMMIO.MetricMinimalMMIOPrimitivesParams, MinimalMMIO.isMMIOAddr,
+        StateMachineMMIOSpec in A.
+    specialize A with (2 := H0). cbv beta in A.
+    inversion H. subst. clear H.
+    destruct A as (A & _). 1: split; assumption.
+    destruct A as (_ & finalH & Pf & Un & Dj).
+
+  Admitted.
+
+  Lemma stateMachine_to_cava: forall (initialH: MetricRiscvMachine) (initialL: ExtraRiscvMachine D)
+                                     steps_done post,
+      related initialH initialL ->
+      runsTo stepH initialH post ->
+      exists steps_remaining finalL finalH,
+        run_rec sched steps_done steps_remaining initialL = (Some tt, finalL) /\
+        related finalH finalL /\
+        post finalH.
+  Proof.
+    intros. revert initialL steps_done H. induction H0; intros.
+    - exists 0%nat. unfold run, run_rec, Monads.Return. simpl. eauto.
+    - pose proof stateMachine_to_cava_1 as One.
+      specialize One with (1 := H2) (2 := H). specialize (One steps_done).
+      destruct One as (midL & midH & One & Rmid & M).
+      specialize H1 with (1 := M) (2 := Rmid). specialize (H1 (S steps_done)).
+      destruct H1 as (steps_remaining & finalL & finalH & Star & Rfinal & Pfinal).
+      exists (S steps_remaining). simpl. rewrite One. eauto.
+  Qed.
+
+End WithParams.
